src/Analysis/Instances/Sign/Sign_Backward.thy
@@ -196,12 +196,96 @@ lemma assume_not_sign_sound:
   unfolding assume_not_sign_def
   using sign_backward_domain.bfilter_sound by simp
 
+
+lemma sign_le_iff:
+  "sign_le a b \<longleftrightarrow> a \<le> b"
+  by (cases a; cases b; auto simp: less_eq_sign_def)
+
+lemma narrow1_mono:
+  fixes x x' y y' c d :: "'a::semilattice_inf"
+  assumes xx': "x \<le> x'"
+      and yy': "y \<le> y'"
+  shows
+    "(if y \<le> c then x \<sqinter> d else x)
+      \<le> (if y' \<le> c then x' \<sqinter> d else x')"
+  using xx' yy' inf_mono
+  by auto
+
+lemma narrow2_mono:
+  fixes x x' y y' c1 c2 :: "'a::semilattice_inf"
+  assumes xx': "x \<le> x'"
+      and yy': "y \<le> y'"
+      and cc': "c1 \<le> c2"
+  shows
+    "(if y \<le> c1 then x \<sqinter> c1
+      else if y \<le> c2 then x \<sqinter> c2
+      else x)
+      \<le>
+     (if y' \<le> c1 then x' \<sqinter> c1
+      else if y' \<le> c2 then x' \<sqinter> c2
+      else x')"
+  using xx' yy' cc' inf_mono
+  by (auto simp add: inf.coboundedI1 inf.coboundedI2)
+
 lemma inv_less_sign_mono:
-  "a1 \<le> (a1'::sign) \<Longrightarrow> a2 \<le> a2' \<Longrightarrow>
-   fst (inv_less_sign r a1 a2) \<le> fst (inv_less_sign r a1' a2') \<and>
-   snd (inv_less_sign r a1 a2) \<le> snd (inv_less_sign r a1' a2')"
-  by (cases r; cases a1; cases a1'; cases a2; cases a2';
-      auto simp: less_eq_sign_def)
+  assumes A1: "a1 \<le> (a1' :: sign)"
+      and A2: "a2 \<le> a2'"
+  shows
+    "fst (inv_less_sign r a1 a2)
+       \<le> fst (inv_less_sign r a1' a2') \<and>
+     snd (inv_less_sign r a1 a2)
+       \<le> snd (inv_less_sign r a1' a2')"
+proof (cases r)
+  case True
+
+  have fst_mono:
+    "(if a2 \<le> SNonPos then a1 \<sqinter> SNeg else a1)
+      \<le>
+     (if a2' \<le> SNonPos then a1' \<sqinter> SNeg else a1')"
+    using narrow1_mono[OF A1 A2, of SNonPos SNeg] .
+
+  have snd_mono:
+    "(if a1 \<le> SNonNeg then a2 \<sqinter> SPos else a2)
+      \<le>
+     (if a1' \<le> SNonNeg then a2' \<sqinter> SPos else a2')"
+    using narrow1_mono[OF A2 A1, of SNonNeg SPos] .
+
+  show ?thesis
+    using fst_mono snd_mono True sign_le_iff
+    by auto
+next
+  case False
+
+  have pos_order: "(SPos :: sign) \<le> SNonNeg"
+    by (simp add: less_eq_sign_def)
+
+  have neg_order: "(SNeg :: sign) \<le> SNonPos"
+    by (simp add: less_eq_sign_def)
+
+  have fst_mono:
+    "(if a2 \<le> SPos then a1 \<sqinter> SPos
+      else if a2 \<le> SNonNeg then a1 \<sqinter> SNonNeg
+      else a1)
+      \<le>  
+     (if a2' \<le> SPos then a1' \<sqinter> SPos
+      else if a2' \<le> SNonNeg then a1' \<sqinter> SNonNeg
+      else a1')"
+    using narrow2_mono[OF A1 A2, of SPos SNonNeg] pos_order by simp
+
+  have snd_mono:
+    "(if a1 \<le> SNeg then a2 \<sqinter> SNeg
+      else if a1 \<le> SNonPos then a2 \<sqinter> SNonPos
+      else a2)
+      \<le>
+     (if a1' \<le> SNeg then a2' \<sqinter> SNeg
+      else if a1' \<le> SNonPos then a2' \<sqinter> SNonPos
+      else a2')"
+    using narrow2_mono[OF A2 A1, of SNeg SNonPos] neg_order by simp
+
+  show ?thesis
+    using fst_mono snd_mono False sign_le_iff
+    by fastforce
+qed
 
 text \<open>
   Monotonicity of @{const afilter_sign} / @{const bfilter_sign} is the generic
@@ -218,11 +302,12 @@ proof unfold_locales
   fix a1 a2 b1 b2 :: sign
   assume "a1 \<le> a2" and "b1 \<le> b2"
   thus "meet_sign a1 b1 \<le> meet_sign a2 b2"
-    by (cases a1; cases a2; cases b1; cases b2; auto simp: less_eq_sign_def)
+    using inf_mono[OF \<open>a1 \<le> a2\<close> \<open>b1 \<le> b2\<close>] by simp
 next
   fix e :: aexp and \<sigma>1 \<sigma>2 :: "vname \<Rightarrow> sign"
   assume "\<sigma>1 \<le> \<sigma>2"
-  thus "aval_sign e \<sigma>1 \<le> aval_sign e \<sigma>2" by (rule aval_sign_mono)
+  thus "  apply(cases r)
+aval_sign e \<sigma>1 \<le> aval_sign e \<sigma>2" by (rule aval_sign_mono)
 next
   fix x1 x2 y1 y2 :: sign and res :: bool
   assume "x1 \<le> x2" and "y1 \<le> y2"
